\documentclass{article}

\usepackage{graphicx}

\begin{document}

\begin{enumerate}

\item \begin{equation} V(r)=D_e(1-\frac{u(r)}{u(r_e)}e^{-\beta(r)y_p^{r_\textrm{eq}}}) \end{equation}

\item \begin{equation} \beta(r)=(1-y_p^{r_\textrm{{ref}}}(r))\sum_{i=0}^{N_\beta}\beta_iy_q^{r_\textrm{{ref}}}(r)^i+y_p^{r_\textrm{{ref}}}(r)\beta_\infty\end{equation}

\item \begin{equation} y_n^{r_x}(r)=\frac{r^n-r_x^n}{r^n+r_x^n} \end{equation}

\item \begin{equation} \ \lim_{r\to\infty} \beta(r) \ = \beta_\infty \end{equation}

\item \begin{equation} \ \lim_{r\to\infty} y_n^{r_x} = 0 \end{equation}

\item \begin{equation} \ \lim_{r\to\infty} -\beta(r)y_p^{r_\textrm{eq}}(r) = \infty \end{equation}



\end{enumerate}

\end{document}